Functor.fsti in new style, too

code/streaming/Hacl.Streaming.Functor.fsti
@@ -18,9 +18,9 @@ module G = FStar.Ghost
 module S = FStar.Seq
 module U32 = FStar.UInt32
 module U64 = FStar.UInt64
-module I = Hacl.Streaming.Interface
 
-open Hacl.Streaming.Interface
+open Hacl.Streaming.Block
+
 open FStar.HyperStack.ST
 open LowStar.BufferOps
 open FStar.Mul
@@ -38,32 +38,32 @@ let uint32 = Lib.IntTypes.uint32
 // and Hacl_Streaming_SHA1.c from compiling, because KaRaMeL tries to share the state_s
 // type definition with Hacl_Streaming_SHA2.c, which is hidden.
 //[@CAbstractStruct]
-val state_s (#index: Type0) (c: block index) (i: index)
-  (t: Type0 { t == c.state.s i })
-  (t': Type0 { t' == optional_key i c.km c.key }):
+val state_s (c: index)
+  (t: Type0 { t == c.state.s })
+  (t': Type0 { t' == optional_key c }):
   Type0
 
 inline_for_extraction noextract
-let state_s' c i = state_s c i (c.state.s i) (optional_key i c.km c.key)
+let state_s' c = state_s c c.state.s (optional_key c)
 
 /// State is equipped with a superfluous type-level parameter to ensure ML-like
 /// prenex polymorphism and hence low-level monomorphization via KaRaMeL.
 ///
 /// Run-time functions MUST take t as a parameter. Proof-level functions are
 /// welcome to instantiate it directly with ``c.state i``.
-let state #index (c: block index) (i: index)
-  (t: Type0 { t == c.state.s i })
-  (t': Type0 { t' == optional_key i c.km c.key })
+let state (c: index)
+  (t: Type0 { t == c.state.s })
+  (t': Type0 { t' == optional_key c})
 =
-  B.pointer (state_s c i t t')
+  B.pointer (state_s c t t')
 
 inline_for_extraction noextract
-let state' c i = state c i (c.state.s i) (optional_key i c.km c.key)
+let state' c = state c c.state.s (optional_key c)
 
-val footprint_s (#index: Type0) (c: block index) (i: index) (h: HS.mem) (s: state_s' c i): GTot B.loc
+val footprint_s (c: index) (h: HS.mem) (s: state_s' c): GTot B.loc
 
-let footprint (#index: Type0) (c: block index) (i: index) (m: HS.mem) (s: state' c i) =
-  B.(loc_union (loc_addr_of_buffer s) (footprint_s c i m (B.deref m s)))
+let footprint (c: index) (m: HS.mem) (s: state' c) =
+  B.(loc_union (loc_addr_of_buffer s) (footprint_s c m (B.deref m s)))
 
 /// Invariants
 /// ==========
@@ -72,45 +72,41 @@ noextract
 let bytes = S.seq uint8
 
 let loc_includes_union_l_footprint_s
-  #index
-  (c: block index)
-  (i: index)
+  (c: index)
   (m: HS.mem)
-  (l1 l2: B.loc) (s: state_s' c i)
+  (l1 l2: B.loc) (s: state_s' c)
 : Lemma
   (requires (
-    B.loc_includes l1 (footprint_s c i m s) \/ B.loc_includes l2 (footprint_s c i m s)
+    B.loc_includes l1 (footprint_s c m s) \/ B.loc_includes l2 (footprint_s c m s)
   ))
-  (ensures (B.loc_includes (B.loc_union l1 l2) (footprint_s c i m s)))
-  [SMTPat (B.loc_includes (B.loc_union l1 l2) (footprint_s c i m s))]
-= B.loc_includes_union_l l1 l2 (footprint_s c i m s)
+  (ensures (B.loc_includes (B.loc_union l1 l2) (footprint_s c m s)))
+  [SMTPat (B.loc_includes (B.loc_union l1 l2) (footprint_s c m s))]
+= B.loc_includes_union_l l1 l2 (footprint_s c m s)
 
 inline_for_extraction noextract
-val invariant_s (#index: Type0) (c: block index) (i: index) (h: HS.mem) (s: state_s' c i): Type0
+val invariant_s (c: index) (h: HS.mem) (s: state_s' c): Type0
 
 inline_for_extraction noextract
-val freeable (#index : Type0) (c: block index) (i: index) (h: HS.mem) (s: state' c i) : Type0
+val freeable (c: index) (h: HS.mem) (s: state' c) : Type0
 
 inline_for_extraction noextract
-let preserves_freeable (#index : Type0) (c: block index) (i: index) (s: state' c i) (h0 h1 : HS.mem): Type0 =
-  freeable c i h0 s ==> freeable c i h1 s
+let preserves_freeable (c: index) (s: state' c) (h0 h1 : HS.mem): Type0 =
+  freeable c h0 s ==> freeable c h1 s
 
 inline_for_extraction noextract
-let invariant #index (c: block index) (i: index) (m: HS.mem) (s: state' c i) =
-  invariant_s c i m (B.get m s 0) /\
+let invariant (c: index) (m: HS.mem) (s: state' c) =
+  invariant_s c m (B.get m s 0) /\
   B.live m s /\
-  B.(loc_disjoint (loc_addr_of_buffer s) (footprint_s c i m (B.deref m s)))
+  B.(loc_disjoint (loc_addr_of_buffer s) (footprint_s c m (B.deref m s)))
 
 val invariant_loc_in_footprint
-  (#index: Type0)
-  (c: block index)
-  (i: index)
-  (s: state' c i)
+  (c: index)
+  (s: state' c)
   (m: HS.mem)
 : Lemma
-  (requires (invariant c i m s))
-  (ensures (B.loc_in (footprint c i m s) m))
-  [SMTPat (invariant c i m s)]
+  (requires (invariant c m s))
+  (ensures (B.loc_in (footprint c m s) m))
+  [SMTPat (invariant c m s)]
 
 /// Keeping track of the bytes fed into the algorithm so far
 /// ========================================================
@@ -156,7 +152,7 @@ val invariant_loc_in_footprint
 ///
 ///                                            JP (20190607)
 
-val seen: #index:Type0 -> c:block index -> i:index -> h:HS.mem -> s:state' c i -> GTot bytes
+val seen: c:index -> h:HS.mem -> s:state' c -> GTot bytes
 
 /// We maintain the invariant that the length of the data hashed so far is smaller
 /// than the maximum length accepted by the hash algorithm.
@@ -165,11 +161,11 @@ val seen: #index:Type0 -> c:block index -> i:index -> h:HS.mem -> s:state' c i -
 /// concatenated with the bytes fed into the algorithm (we copy this iniial
 /// block into the temporary buffer upon initilization). We count the length of
 /// this initial block in the total length of the hashed data.
-val seen_bounded: #index:Type0 -> c:block index -> i:index -> h:HS.mem -> s:state' c i -> Lemma
+val seen_bounded: c:index -> h:HS.mem -> s:state' c -> Lemma
   (requires (
-    invariant c i h s))
+    invariant c h s))
   (ensures (
-    U32.v (c.init_input_len i) + S.length (seen c i h s) <= U64.v (c.max_input_len i)))
+    U32.v c.init_input_len + S.length (seen c h s) <= U64.v c.max_input_len))
 
 /// A fine design point here... There are two styles that have been used in
 /// EverCrypt and throughout for key management.
@@ -186,7 +182,7 @@ val seen_bounded: #index:Type0 -> c:block index -> i:index -> h:HS.mem -> s:stat
 /// key remains the same (i.e. we specify it fully just like ``seen``).
 ///
 /// Note: annotating the projector because of an interleaving bug.
-val key: #index:Type0 -> c:block index -> i:index -> h:HS.mem -> s:state' c i -> GTot (c.key.I.t i)
+val key: c:index -> h:HS.mem -> s:state' c -> GTot c.key.t
 
 /// Framing
 /// =======
@@ -203,270 +199,227 @@ val key: #index:Type0 -> c:block index -> i:index -> h:HS.mem -> s:state' c i ->
 ///
 /// TODO: frame_key!
 
-val frame_invariant: #index:Type0 -> c:block index -> i:index -> l:B.loc -> s:state' c i -> h0:HS.mem -> h1:HS.mem -> Lemma
+val frame_invariant: c:index -> l:B.loc -> s:state' c -> h0:HS.mem -> h1:HS.mem -> Lemma
   (requires (
-    invariant c i h0 s /\
-    B.loc_disjoint l (footprint c i h0 s) /\
+    invariant c h0 s /\
+    B.loc_disjoint l (footprint c h0 s) /\
     B.modifies l h0 h1))
   (ensures (
-    invariant c i h1 s /\
-    footprint c i h0 s == footprint c i h1 s /\
-    preserves_freeable c i s h0 h1))
-  [ SMTPat (invariant c i h1 s); SMTPat (B.modifies l h0 h1) ]
+    invariant c h1 s /\
+    footprint c h0 s == footprint c h1 s /\
+    preserves_freeable c s h0 h1))
+  [ SMTPat (invariant c h1 s); SMTPat (B.modifies l h0 h1) ]
 
-val frame_seen: #index:Type0 -> c:block index -> i:index -> l:B.loc -> s:state' c i -> h0:HS.mem -> h1:HS.mem -> Lemma
+val frame_seen: c:index -> l:B.loc -> s:state' c -> h0:HS.mem -> h1:HS.mem -> Lemma
   (requires (
-    invariant c i h0 s /\
-    B.loc_disjoint l (footprint c i h0 s) /\
+    invariant c h0 s /\
+    B.loc_disjoint l (footprint c h0 s) /\
     B.modifies l h0 h1))
-  (ensures (seen c i h0 s == seen c i h1 s))
-  [ SMTPat (seen c i h1 s); SMTPat (B.modifies l h0 h1) ]
+  (ensures (seen c h0 s == seen c h1 s))
+  [ SMTPat (seen c h1 s); SMTPat (B.modifies l h0 h1) ]
 
 
 /// Stateful API
 /// ============
 
-inline_for_extraction noextract
-val index_of_state:
-  #index:Type0 ->
-  c:block index ->
-  i:G.erased index -> (
-  let i = G.reveal i in
-  t:Type0 { t == c.state.s i } ->
-  t':Type0 { t' == optional_key i c.km c.key } ->
-  s:state c i t t' ->
-  Stack index
-  (fun h0 -> invariant c i h0 s)
-  (fun h0 i' h1 -> h0 == h1 /\ i' == i))
-
 // The number of bytes fed so far into the hash, so that the client doesn't have
 // to track it themselves, since this module does it anyhow.
 inline_for_extraction noextract
 val seen_length:
-  #index:Type0 ->
-  c:block index ->
-  i:G.erased index -> (
-  let i = G.reveal i in
-  t:Type0 { t == c.state.s i } ->
-  t':Type0 { t' == optional_key i c.km c.key } ->
-  s:state c i t t' ->
+  c:index ->
+  t:Type0 { t == c.state.s } ->
+  t':Type0 { t' == optional_key c } ->
+  s:state c t t' ->
   Stack U64.t
-  (fun h0 -> invariant c i h0 s)
-  (fun h0 l h1 -> h0 == h1 /\ U64.v l == U32.v (c.init_input_len i) +  S.length (seen c i h0 s)))
+  (fun h0 -> invariant c h0 s)
+  (fun h0 l h1 -> h0 == h1 /\ U64.v l == U32.v c.init_input_len +  S.length (seen c h0 s))
 
 inline_for_extraction noextract
 let create_in_st
-  (#index: Type0)
-  (c:block index)
-  (i:index)
-  (t:Type0 { t == c.state.s i })
-  (t':Type0 { t' == optional_key i c.km c.key }) =
-  k:c.key.s i ->
+  (c:index)
+  (t:Type0 { t == c.state.s })
+  (t':Type0 { t' == optional_key c }) =
+  k:c.key.s ->
   r: HS.rid ->
-  ST (state c i t t')
+  ST (state c t t')
   (requires (fun h0 ->
-    c.key.invariant #i h0 k /\
+    c.key.invariant h0 k /\
     HyperStack.ST.is_eternal_region r))
   (ensures (fun h0 s h1 ->
-    invariant c i h1 s /\
-    freeable c i h1 s /\
-    seen c i h1 s == S.empty /\
-    key c i h1 s == c.key.v i h0 k /\
+    invariant c h1 s /\
+    freeable c h1 s /\
+    seen c h1 s == S.empty /\
+    key c h1 s == c.key.v h0 k /\
     B.(modifies loc_none h0 h1) /\
-    B.fresh_loc (footprint c i h1 s) h0 h1 /\
-    B.(loc_includes (loc_region_only true r) (footprint c i h1 s))))
+    B.fresh_loc (footprint c h1 s) h0 h1 /\
+    B.(loc_includes (loc_region_only true r) (footprint c h1 s))))
 
 inline_for_extraction noextract
 val create_in:
-  #index: Type0 ->
-  c:block index ->
-  i:index ->
-  t:Type0 { t == c.state.s i } ->
-  t':Type0 { t' == optional_key i c.km c.key } ->
-  create_in_st c i t t'
+  c:index ->
+  t:Type0 { t == c.state.s } ->
+  t':Type0 { t' == optional_key c } ->
+  create_in_st c t t'
 
 inline_for_extraction noextract
 let copy_st
-  (#index: Type0)
-  (c:block index)
-  (i:index)
-  (t:Type0 { t == c.state.s i })
-  (t':Type0 { t' == optional_key i c.km c.key }) =
-  s0:state c i t t' ->
+  (c:index)
+  (t:Type0 { t == c.state.s })
+  (t':Type0 { t' == optional_key c }) =
+  s0:state c t t' ->
   r: HS.rid ->
-  ST (state c i t t')
+  ST (state c t t')
   (requires (fun h0 ->
-    invariant c i h0 s0 /\
+    invariant c h0 s0 /\
     HyperStack.ST.is_eternal_region r))
   (ensures (fun h0 s h1 ->
-    invariant c i h1 s /\
-    freeable c i h1 s /\
-    seen c i h1 s == seen c i h0 s0 /\
-    key c i h1 s == key c i h0 s0 /\
+    invariant c h1 s /\
+    freeable c h1 s /\
+    seen c h1 s == seen c h0 s0 /\
+    key c h1 s == key c h0 s0 /\
     B.(modifies loc_none h0 h1) /\
-    B.fresh_loc (footprint c i h1 s) h0 h1 /\
-    B.(loc_includes (loc_region_only true r) (footprint c i h1 s))))
+    B.fresh_loc (footprint c h1 s) h0 h1 /\
+    B.(loc_includes (loc_region_only true r) (footprint c h1 s))))
 
 inline_for_extraction noextract
 val copy:
-  #index: Type0 ->
-  c:block index ->
-  i:G.erased index ->
-  t:Type0 { t == c.state.s i } ->
-  t':Type0 { t' == optional_key (G.reveal i) c.km c.key } ->
-  copy_st c i t t'
+  c:G.erased index ->
+  t:Type0 { t == c.state.s } ->
+  t':Type0 { t' == optional_key c } ->
+  copy_st c t t'
 
 inline_for_extraction noextract
 let alloca_st
-  (#index: Type0)
-  (c:block index)
-  (i:index)
-  (t:Type0 { t == c.state.s i })
-  (t':Type0 { t' == optional_key i c.km c.key }) =
-  k:c.key.s i ->
-  StackInline (state c i t t')
+  (c:index)
+  (t:Type0 { t == c.state.s })
+  (t':Type0 { t' == optional_key c }) =
+  k:c.key.s ->
+  StackInline (state c t t')
   (requires (fun h0 ->
-    c.key.invariant #i h0 k))
+    c.key.invariant h0 k))
   (ensures (fun h0 s h1 ->
-    invariant c i h1 s /\
-    seen c i h1 s == S.empty /\
-    key c i h1 s == c.key.v i h0 k /\
+    invariant c h1 s /\
+    seen c h1 s == S.empty /\
+    key c h1 s == c.key.v h0 k /\
     B.(modifies loc_none h0 h1) /\
-    B.fresh_loc (footprint c i h1 s) h0 h1 /\
-    B.(loc_includes (loc_region_only true (HS.get_tip h1)) (footprint c i h1 s))))
+    B.fresh_loc (footprint c h1 s) h0 h1 /\
+    B.(loc_includes (loc_region_only true (HS.get_tip h1)) (footprint c h1 s))))
 
 inline_for_extraction noextract
 val alloca:
-  #index: Type0 ->
-  c:block index ->
-  i:index ->
-  t:Type0 { t == c.state.s i } ->
-  t':Type0 { t' == optional_key i c.km c.key } ->
-  alloca_st #index c i t t'
+  c:index ->
+  t:Type0 { t == c.state.s } ->
+  t':Type0 { t' == optional_key c } ->
+  alloca_st c t t'
 
 /// Note: this is more like a "reinit" function so that clients can reuse the state.
 inline_for_extraction noextract
 let init_st
-  (#index: Type0)
-  (c:block index)
-  (i:G.erased index)
-  (t:Type0 { t == c.state.s i })
-  (t':Type0 { t' == optional_key (G.reveal i) c.km c.key }) =
-  k:c.key.s i ->
-  s:state c i t t' ->
+  (c:G.erased index)
+  (t:Type0 { t == c.state.s })
+  (t':Type0 { t' == optional_key c }) =
+  k:c.key.s ->
+  s:state c t t' ->
   Stack unit
   (requires (fun h0 ->
-    c.key.invariant #i h0 k /\
-    B.loc_disjoint (c.key.footprint #i h0 k) (footprint c i h0 s) /\
-    invariant c i h0 s))
+    c.key.invariant h0 k /\
+    B.loc_disjoint (c.key.footprint h0 k) (footprint c h0 s) /\
+    invariant c h0 s))
   (ensures (fun h0 _ h1 ->
-    invariant c i h1 s /\
-    seen c i h1 s == S.empty /\
-    key c i h1 s == c.key.v i h0 k /\
-    footprint c i h0 s == footprint c i h1 s /\
-    B.(modifies (footprint c i h0 s) h0 h1) /\
-    preserves_freeable c i s h0 h1))
+    invariant c h1 s /\
+    seen c h1 s == S.empty /\
+    key c h1 s == c.key.v h0 k /\
+    footprint c h0 s == footprint c h1 s /\
+    B.(modifies (footprint c h0 s) h0 h1) /\
+    preserves_freeable c s h0 h1))
 
 inline_for_extraction noextract
 val init:
-  #index:Type0 ->
-  c:block index ->
-  i:G.erased index -> (
-  let i = G.reveal i in
-  t:Type0 { t == c.state.s i } ->
-  t':Type0 { t' == optional_key i c.km c.key } ->
-  init_st #index c i t t')
+  c:G.erased index ->
+  t:Type0 { t == c.state.s } ->
+  t':Type0 { t' == optional_key c } ->
+  init_st c t t'
 
 unfold noextract
 let update_pre
-  #index
-  (c: block index)
-  (i: index)
-  (s: state' c i)
+  (c: index)
+  (s: state' c)
   (data: B.buffer uint8)
   (len: UInt32.t)
   (h0: HS.mem)
 =
-  invariant c i h0 s /\
+  invariant c h0 s /\
   B.live h0 data /\
   U32.v len = B.length data /\
-  B.(loc_disjoint (loc_buffer data) (footprint c i h0 s))
+  B.(loc_disjoint (loc_buffer data) (footprint c h0 s))
 
 unfold noextract
 let update_post
-  #index
-  (c: block index)
-  (i: index)
-  (s: state' c i)
+  (c: index)
+  (s: state' c)
   (data: B.buffer uint8)
   (len: UInt32.t)
   (h0 h1: HS.mem)
 =
-  invariant c i h1 s /\
-  B.(modifies (footprint c i h0 s) h0 h1) /\
-  footprint c i h0 s == footprint c i h1 s /\
-  seen c i h1 s == seen c i h0 s `S.append` B.as_seq h0 data /\
-  key c i h1 s == key c i h0 s /\
-  preserves_freeable c i s h0 h1
+  invariant c h1 s /\
+  B.(modifies (footprint c h0 s) h0 h1) /\
+  footprint c h0 s == footprint c h1 s /\
+  seen c h1 s == seen c h0 s `S.append` B.as_seq h0 data /\
+  key c h1 s == key c h0 s /\
+  preserves_freeable c s h0 h1
 
 inline_for_extraction noextract
 let update_st
-  (#index: Type0)
-  (c:block index)
-  (i:index)
-  (t:Type0 { t == c.state.s i })
-  (t':Type0 { t' == optional_key i c.km c.key }) =
-  s:state c i t t' ->
+  (c:index)
+  (t:Type0 { t == c.state.s })
+  (t':Type0 { t' == optional_key c }) =
+  s:state c t t' ->
   data: B.buffer uint8 ->
   len: UInt32.t ->
   Stack Hacl.Streaming.Types.error_code
-    (requires fun h0 -> update_pre c i s data len h0)
+    (requires fun h0 -> update_pre c s data len h0)
     (ensures fun h0 s' h1 ->
       let open Hacl.Streaming.Types in
       match s' with
       | Success ->
-          U32.v (c.init_input_len i) + S.length (seen c i h0 s) + UInt32.v len <= U64.v (c.max_input_len i) /\
-          update_post c i s data len h0 h1
+          U32.v c.init_input_len + S.length (seen c h0 s) + UInt32.v len <= U64.v c.max_input_len /\
+          update_post c s data len h0 h1
       | MaximumLengthExceeded ->
-          U32.v (c.init_input_len i) + S.length (seen c i h0 s) + UInt32.v len > U64.v (c.max_input_len i) /\
+          U32.v c.init_input_len + S.length (seen c h0 s) + UInt32.v len > U64.v c.max_input_len /\
           h0 == h1
       | _ ->
           False)
 
 inline_for_extraction noextract
 val update:
-  #index:Type0 ->
-  c:block index ->
-  i:G.erased index -> (
-  let i = G.reveal i in
-  t:Type0 { t == c.state.s i } ->
-  t':Type0 { t' == optional_key i c.km c.key } ->
-  update_st #index c i t t')
+  c:G.erased index ->
+  t:Type0 { t == c.state.s } ->
+  t':Type0 { t' == optional_key c } ->
+  update_st c t t'
+
 
 inline_for_extraction noextract
 let finish_st
-  #index
-  (c: block index)
-  (i: index)
-  (t: Type0 { t == c.state.s i })
-  (t':Type0 { t' == optional_key i c.km c.key }) =
-  s:state c i t t' ->
+  (c: index)
+  (t: Type0 { t == c.state.s })
+  (t':Type0 { t' == optional_key c }) =
+  s:state c t t' ->
   dst:B.buffer uint8 ->
-  l:c.output_length_t { B.length dst == c.output_length i l } ->
+  l:c.output_length_t { B.length dst == c.output_length l } ->
   Stack unit
     (requires fun h0 ->
-      invariant c i h0 s /\
+      invariant c h0 s /\
       B.live h0 dst /\
-      B.(loc_disjoint (loc_buffer dst) (footprint c i h0 s)))
+      B.(loc_disjoint (loc_buffer dst) (footprint c h0 s)))
     (ensures fun h0 s' h1 ->
-      invariant c i h1 s /\
-      seen c i h0 s == seen c i h1 s /\
-      key c i h1 s == key c i h0 s /\
-      footprint c i h0 s == footprint c i h1 s /\
-      B.(modifies (loc_union (loc_buffer dst) (footprint c i h0 s)) h0 h1) /\ (
-      seen_bounded c i h0 s;
-      S.equal (B.as_seq h1 dst) (c.spec_s i (key c i h0 s) (seen c i h0 s) l)) /\
-      preserves_freeable c i s h0 h1)
+      invariant c h1 s /\
+      seen c h0 s == seen c h1 s /\
+      key c h1 s == key c h0 s /\
+      footprint c h0 s == footprint c h1 s /\
+      B.(modifies (loc_union (loc_buffer dst) (footprint c h0 s)) h0 h1) /\ (
+      seen_bounded c h0 s;
+      S.equal (B.as_seq h1 dst) (c.spec_s (key c h0 s) (seen c h0 s) l)) /\
+      preserves_freeable c s h0 h1)
 
 /// A word of caution. Once partially applied to a type class, this function
 /// will generate a stack allocation at type ``state i`` via ``c.alloca``. If
@@ -480,34 +433,27 @@ let finish_st
 /// and does not need to be specialized.
 inline_for_extraction noextract
 val mk_finish:
-  #index:Type0 ->
-  c:block index ->
-  i:index ->
-  t:Type0 { t == c.state.s i } ->
-  t':Type0 { t' == optional_key (G.reveal i) c.km c.key } ->
-  finish_st c i t t'
+  c:index ->
+  t:Type0 { t == c.state.s } ->
+  t':Type0 { t' == optional_key c } ->
+  finish_st c t t'
 
 inline_for_extraction noextract
 let free_st
-  (#index: Type0)
-  (c:block index)
-  (i:index)
-  (t:Type0 { t == c.state.s i })
-  (t':Type0 { t' == optional_key i c.km c.key }) =
-  s:state c i t t' ->
+  (c:index)
+  (t:Type0 { t == c.state.s })
+  (t':Type0 { t' == optional_key c }) =
+  s:state c t t' ->
   ST unit
   (requires fun h0 ->
-    invariant c i h0 s /\
-    freeable c i h0 s)
+    invariant c h0 s /\
+    freeable c h0 s)
   (ensures fun h0 _ h1 ->
-    B.modifies (footprint c i h0 s) h0 h1)
+    B.modifies (footprint c h0 s) h0 h1)
 
 inline_for_extraction noextract
 val free:
-  #index:Type0 ->
-  c:block index ->
-  i:G.erased index -> (
-  let i = G.reveal i in
-  t:Type0 { t == c.state.s i } ->
-  t':Type0 { t' == optional_key i c.km c.key } ->
-  free_st #index c i t t')
+  c:index ->
+  t:Type0 { t == c.state.s } ->
+  t':Type0 { t' == optional_key c } ->
+  free_st c t t'
